chore(library/init): remove coroutines from stdlib

tests/lean/run/coroutine.lean
@@ -1,6 +1,147 @@
-import init.control.coroutine
+universes u v w r s
 
-universes u v
+inductive coroutine_result_core (coroutine : Type (max u v w)) (α : Type u) (δ : Type v) (β : Type w) : Type (max u v w)
+| done     {} : β → coroutine_result_core
+| yielded {}  : δ → coroutine → coroutine_result_core
+
+/--
+   Asymmetric coroutines `coroutine α δ β` takes inputs of type `α`, yields elements of type `δ`,
+   and produces an element of type `β`.
+
+   Asymmetric coroutines are so called because they involve two types of control transfer operations:
+   one for resuming/invoking a coroutine and one for suspending it, the latter returning
+   control to the coroutine invoker. An asymmetric coroutine can be regarded as subordinate
+   to its caller, the relationship between them being similar to that between a called and
+   a calling routine.
+ -/
+inductive coroutine (α : Type u) (δ : Type v) (β : Type w) : Type (max u v w)
+| mk    {} : (α → coroutine_result_core coroutine α δ β) → coroutine
+
+abbreviation coroutine_result (α : Type u) (δ : Type v) (β : Type w) : Type (max u v w) :=
+coroutine_result_core (coroutine α δ β) α δ β
+
+namespace coroutine
+variables {α : Type u} {δ : Type v} {β γ : Type w}
+
+export coroutine_result_core (done yielded)
+
+/-- `resume c a` resumes/invokes the coroutine `c` with input `a`. -/
+@[inline] def resume : coroutine α δ β → α → coroutine_result α δ β
+| (mk k) a := k a
+
+@[inline] protected def pure (b : β) : coroutine α δ β :=
+mk $ λ _, done b
+
+/-- Read the input argument passed to the coroutine.
+    Remark: should we use a different name? I added an instance [monad_reader] later. -/
+@[inline] protected def read : coroutine α δ α :=
+mk $ λ a, done a
+
+/-- Run nested coroutine with transformed input argument. Like `reader_t.adapt`, but
+    cannot change the input type. -/
+@[inline] protected def adapt (f : α → α) (c : coroutine α δ β) : coroutine α δ β :=
+mk $ λ a, c.resume (f a)
+
+/-- Return the control to the invoker with result `d` -/
+@[inline] protected def yield (d : δ) : coroutine α δ punit :=
+mk $ λ a : α, yielded d (coroutine.pure ⟨⟩)
+
+/-
+TODO(Leo): following relations have been commented because Lean4 is currently
+accepting non-terminating programs.
+
+/-- Auxiliary relation for showing that bind/pipe terminate -/
+inductive direct_subcoroutine : coroutine α δ β → coroutine α δ β → Prop
+| mk : ∀ (k : α → coroutine_result α δ β) (a : α) (d : δ) (c : coroutine α δ β), k a = yielded d c → direct_subcoroutine c (mk k)
+
+theorem direct_subcoroutine_wf : well_founded (@direct_subcoroutine α δ β) :=
+begin
+  constructor, intro c,
+  apply @coroutine.ind _ _ _
+          (λ c, acc direct_subcoroutine c)
+          (λ r, ∀ (d : δ) (c : coroutine α δ β), r = yielded d c → acc direct_subcoroutine c),
+  { intros k ih, dsimp at ih, constructor, intros c' h, cases h, apply ih h_a h_d, assumption },
+  { intros, contradiction },
+  { intros d c ih d₁ c₁ heq, injection heq, subst c, assumption }
+end
+
+/-- Transitive closure of direct_subcoroutine. It is not used here, but may be useful when defining
+    more complex procedures. -/
+def subcoroutine : coroutine α δ β → coroutine α δ β → Prop :=
+tc direct_subcoroutine
+
+theorem subcoroutine_wf : well_founded (@subcoroutine α δ β) :=
+tc.wf direct_subcoroutine_wf
+
+-- Local instances for proving termination by well founded relation
+
+def bind_wf_inst : has_well_founded (Σ' a : coroutine α δ β, (β → coroutine α δ γ)) :=
+{ r  := psigma.lex direct_subcoroutine (λ _, empty_relation),
+  wf := psigma.lex_wf direct_subcoroutine_wf (λ _, empty_wf) }
+
+def pipe_wf_inst : has_well_founded (Σ' a : coroutine α δ β, coroutine δ γ β) :=
+{ r  := psigma.lex direct_subcoroutine (λ _, empty_relation),
+  wf := psigma.lex_wf direct_subcoroutine_wf (λ _, empty_wf) }
+
+local attribute [instance] wf_inst₁ wf_inst₂
+
+open well_founded_tactics
+
+-/
+
+@[inline_if_reduce] protected def bind : coroutine α δ β → (β → coroutine α δ γ) → coroutine α δ γ
+| (mk k) f := mk $ λ a,
+    match k a, rfl : ∀ (n : _), n = k a → _ with
+    | done b, _      := coroutine.resume (f b) a
+    | yielded d c, h :=
+      -- have direct_subcoroutine c (mk k), { apply direct_subcoroutine.mk k a d, rw h },
+      yielded d (bind c f)
+--  using_well_founded { dec_tac := unfold_wf_rel >> process_lex (tactic.assumption) }
+
+def pipe : coroutine α δ β → coroutine δ γ β → coroutine α γ β
+| (mk k₁) (mk k₂) := mk $ λ a,
+  match k₁ a, rfl : ∀ (n : _), n = k₁ a → _ with
+  | done b, h        := done b
+  | yielded d k₁', h :=
+    match k₂ d with
+    | done b        := done b
+    | yielded r k₂' :=
+      -- have direct_subcoroutine k₁' (mk k₁), { apply direct_subcoroutine.mk k₁ a d, rw h },
+      yielded r (pipe k₁' k₂')
+-- using_well_founded { dec_tac := unfold_wf_rel >> process_lex (tactic.assumption) }
+
+private def finish_aux (f : δ → α) : coroutine α δ β → α → list δ → list δ × β
+| (mk k) a ds :=
+  match k a with
+  | done b       := (ds.reverse, b)
+  | yielded d k' := finish_aux k' (f d) (d::ds)
+
+/-- Run a coroutine to completion, feeding back yielded items after transforming them with `f`. -/
+def finish (f : δ → α) : coroutine α δ β → α → list δ × β :=
+λ k a, finish_aux f k a []
+
+instance : monad (coroutine α δ) :=
+{ pure := @coroutine.pure _ _,
+  bind := @coroutine.bind _ _ }
+
+instance : monad_reader α (coroutine α δ) :=
+{ read := @coroutine.read _ _ }
+
+end coroutine
+
+/-- Auxiliary class for lifiting `yield` -/
+class monad_coroutine (α : out_param (Type u)) (δ : out_param (Type v)) (m : Type w → Type r) :=
+(yield {} : δ → m punit)
+
+instance (α : Type u) (δ : Type v) : monad_coroutine α δ (coroutine α δ) :=
+{ yield  := coroutine.yield }
+
+instance monad_coroutine_trans (α : Type u) (δ : Type v) (m : Type w → Type r) (n : Type w → Type s)
+                               [has_monad_lift m n] [monad_coroutine α δ m] : monad_coroutine α δ n :=
+{ yield := λ d, monad_lift (monad_coroutine.yield d : m _) }
+
+export monad_coroutine (yield)
+
 open coroutine
 
 namespace ex1
@@ -55,31 +196,5 @@ do let c := state_t.run ex 5,
    pure ()
 
 #eval tst2
-
-def ex3 : except_t string (coroutine_io nat string) unit :=
-do
-  x ← read,
-  io.println $ "got " ++ to_string x,
-  yield ("1) val: " ++ to_string x),
-  x ← read,
-  io.println $ "got " ++ to_string x,
-  yield ("2) val: " ++ to_string x),
-  throw "my_error"
-
-open coroutine_io
-def tst3 : except_t string io unit :=
-do let c := ex3.run,
-   (yielded r c₁) ← monad_lift $ c.resume 10,
-   io.println r,
-   (yielded r c₂) ← monad_lift $ c₁.resume 20,
-   io.println r,
-   (done (except.error e)) ← monad_lift $ c₂.resume 30,
-   io.println $ "error: " ++ e,
-   (yielded r c₃) ← monad_lift $ c₁.resume 100,
-   io.println r,
-   io.println "done",
-   pure ()
-
-#eval tst3
 
 end ex2
